theories/L/Complexity/Cook/BinaryPR_to_FSAT_extraction.v
@@ -1,0 +1,15 @@
+From Undecidability.L.Complexity.Cook Require Import FlatPR BinaryPR FSAT BinaryPR_to_FSAT.
+
+From Undecidability.L.Tactics Require Import LTactics GenEncode.
+From Undecidability.L.Datatypes Require Import LProd LOptions LBool LLNat LLists LSum.
+From Undecidability.L.Complexity Require Import PolyBounds. 
+
+
+(** encodeLiteral *)
+Definition c__encodeLiteral := 1.
+Instance term_encodeLiteral : computableTime' encodeLiteral (fun v _ => (1, fun s _ => (c__encodeLiteral, tt))). 
+Proof. 
+  (*TODO: simplification fails. why!? *)
+  extract. 
+Admitted. 
+
