theories/L/Complexity/Cook/FlatGenNP_to_FlatTPR.v
@@ -1,0 +1,200 @@
+From Undecidability.L.Complexity.Cook Require Import Prelim GenNP_PR FlatTPR FlatFinTypes FlatFinTypes_extraction. 
+
+From Undecidability.L.Tactics Require Import LTactics GenEncode.
+From Undecidability.L.Datatypes Require Import LProd LOptions LBool LLNat LLists LSum.
+From Undecidability.L.Complexity Require Import PolyBounds. 
+From Undecidability.L.TM Require Import TMflatEnc TMflat TMEncoding. 
+
+
+(** * extraction of the reduction from FlatGenNP to FlatPR *)
+
+Run TemplateProgram (tmGenEncode "fstateSigma_enc" fstateSigma).
+Hint Resolve fstateSigma_enc_correct : Lrewrite.
+
+Run TemplateProgram (tmGenEncode "fpolarity_enc" fpolarity).
+Hint Resolve fpolarity_enc_correct : Lrewrite. 
+
+Run TemplateProgram (tmGenEncode "fpreludeSig'_enc" fpreludeSig').
+Hint Resolve fpreludeSig'_enc_correct : Lrewrite. 
+
+Run TemplateProgram (tmGenEncode "evalEnv_enc" (evalEnv nat nat nat nat)).
+Hint Resolve evalEnv_enc_correct : Lrewrite. 
+
+Instance term_Build_evalEnv : computableTime' (@Build_evalEnv nat nat nat nat) (fun _ _ => (1, fun _ _ => (1, fun _ _ => (1, fun _ _ => (1, tt))))). 
+Proof. 
+  extract constructor. solverec. 
+Defined. 
+
+Definition c__polarityEnv := 7. 
+Instance term_polarityEnv : computableTime' (@polarityEnv nat nat nat nat) (fun _ _ => (c__polarityEnv, tt)). 
+Proof. 
+  extract. solverec. unfold c__polarityEnv. solverec. 
+Defined. 
+
+Definition c__sigmaEnv := 7.
+Instance term_sigmaEnv : computableTime' (@sigmaEnv nat nat nat nat) (fun _ _ => (c__sigmaEnv, tt)). 
+Proof. 
+  extract. solverec. unfold c__sigmaEnv. solverec. 
+Defined. 
+
+Definition c__stateSigmaEnv := 7.
+Instance term_stateSigmaEnv : computableTime' (@stateSigmaEnv nat nat nat nat) (fun _ _ => (c__stateSigmaEnv, tt)). 
+Proof. 
+  extract. solverec. unfold c__stateSigmaEnv. solverec. 
+Defined. 
+
+Definition c__stateEnv := 7.
+Instance term_stateEnv : computableTime' (@stateEnv nat nat nat nat) (fun _ _ => (c__stateEnv, tt)). 
+Proof. 
+  extract. solverec. unfold c__stateEnv. solverec. 
+Defined. 
+
+Definition c__flattenPolarity := 11.
+Instance term_flattenPolarity : computableTime' flattenPolarity (fun p _ => (c__flattenPolarity, tt)). 
+Proof. 
+  assert (extEq (fun p => match p with TM.L => 0 | TM.R => 1 | TM.N => 2 end) flattenPolarity ) as H. 
+  { intros []; easy. }
+  eapply (computableTimeExt H).
+  extract. solverec. all: now unfold c__flattenPolarity.
+Defined.
+
+(*define notations again, because Coq doesn't allow to keep notations beyond the end of a section (why!?) *)
+Notation fpolSigma  := (prod fpolarity fstateSigma).
+Notation ftapeSigma := (sum delim fpolSigma).
+Notation fStates := (prod nat fstateSigma).
+Notation fGamma := (sum fStates ftapeSigma).
+Notation fAlphabet := (sum fGamma fpreludeSig'). 
+
+(*reifyPolarityFlat *)
+Definition c__reifyPolarityFlat := c__flattenPolarity + c__polarityEnv + 10.
+Definition reifyPolarityFlat_time (env : evalEnvFlat) (p : fpolarity) := 
+  match p with polConst _ =>  0 | polVar n => nth_error_time (polarityEnv env) n end + c__reifyPolarityFlat.
+Instance term_reifyPolarityFlat : computableTime' reifyPolarityFlat (fun env _ => (1, fun p _ => (reifyPolarityFlat_time env p, tt))). 
+Proof. 
+  extract. solverec. 
+  all: unfold reifyPolarityFlat_time, c__reifyPolarityFlat; solverec. 
+Defined. 
+
+(*option_map *)
+Section fix_option_map.
+  Variable (A B : Type).
+  Context `{A_int : registered A}.
+  Context `{B_int : registered B}. 
+
+  Definition c__optionMap := 6.
+  Definition optionMap_time (fT : A -> nat) (a : option A) := match a with None => 0 | Some a => fT a end + c__optionMap.
+  Global Instance term_option_map : computableTime' (@option_map A B) (fun f fT => (1, fun o _ => (optionMap_time (callTime fT) o, tt))). 
+  Proof. 
+    extract. solverec. 
+    all: unfold optionMap_time, c__optionMap; solverec. 
+  Defined. 
+End fix_option_map. 
+
+(*reifyStateSigmaFlat *)
+Definition c__reifyStateSigmaFlat := 15 + c__optionMap + c__sigmaEnv + c__stateSigmaEnv.
+Definition reifyStateSigmaFlat_time (env : evalEnvFlat) (c : fstateSigma) :=  
+  match c with 
+  | blank => 0 
+  | someSigmaVar v => nth_error_time (sigmaEnv env) v 
+  | stateSigmaVar v => nth_error_time (stateSigmaEnv env) v 
+  end + c__reifyStateSigmaFlat.
+Instance term_reifyStateSigmaFlat : computableTime' reifyStateSigmaFlat (fun env _ => (1, fun c _ => (reifyStateSigmaFlat_time env c, tt))). 
+Proof. 
+  extract. solverec. 
+  2: unfold optionMap_time; destruct nth_error. 
+  all: unfold reifyStateSigmaFlat_time, c__reifyStateSigmaFlat; solverec. 
+Defined. 
+
+
+
+(*optBind & optReturn*)
+Section fix_optBind.
+  Variable (X Y : Type).
+  Context `{intX : registered X}.
+  Context `{intY : registered Y}.
+
+  (*Definition optBind_time (fT : X -> nat) (a : option X) := 1. *)
+  (*Global Instance term_optBind : computableTime' (@optBind X Y) (fun a _ => (1, fun f fT => (optBind_time (callTime fT) a, tt))). *)
+  (*Proof. *)
+    (*extract. solverec. *)
+    (*match optBind*)
+
+  (*optReturn*)
+  Global Instance term_optReturn : computableTime' (@optReturn X) (fun a _ => (1, tt)). 
+  Proof. 
+    extract. solverec. 
+  Defined. 
+End fix_optBind. 
+  
+Definition test := fun (flatTM : TM) (env : evalEnvFlat) (c : fpolSigma) =>
+   let (p, s) := c in
+   match reifyPolarityFlat env p with
+   | Some x =>
+       match reifyStateSigmaFlat env s with
+       | Some x0 =>
+           optReturn (flatPair flatPolarity (flatOption (sig flatTM)) x x0)
+       | None => None
+       end
+   | None => None
+   end. 
+
+From Undecidability.L.TM Require Import TMflatEnc TMflat TMEncoding. 
+
+Require Import Undecidability.L.Tactics.ComputableTactics.
+Import ComputableTactics.Intern.
+Definition reifyPolSigmaFlat_time (env : evalEnvFlat) (c : fpolSigma) := 1. 
+Instance term_test : computableTime' test (fun tm _ => (1, fun env _ => (1, fun c _ => (reifyPolSigmaFlat_time env c, tt)))).
+Proof.
+  unfold test. extract. extractAs t. computable_using_noProof t. cstep.
+  cstep. cstep. cstep. cstep. cstep. cstep. unfold optReturn. cstep. 2: cstep. 
+
+Instance term_reifyPolSigmaFlat : computableTime' reifyPolSigmaFlat (fun tm _ => (1, fun env _ => (1, fun c _ => (reifyPolSigmaFlat_time env c, tt)))). 
+Proof. 
+  unfold reifyPolSigmaFlat. unfold optBind. 
+  extract. solverec. 
+
+
+
+  Definition reifyPolSigmaFlat (env : evalEnvFlat) (c : fpolSigma) :=
+    match c with
+    | (p, s) => do p <- reifyPolarityFlat env p;
+                do s <- reifyStateSigmaFlat env s;
+                optReturn (flatPair flatPolarity flatStateSigma p s)
+    end. 
+
+  Definition reifyTapeSigmaFlat (env : evalEnvFlat) (c : ftapeSigma) :=
+    match c with
+    | inl delimC => Some (flatDelimC)
+    | inr c => option_map (flatInr flatDelim) (reifyPolSigmaFlat env c)
+    end.
+
+  Definition reifyStatesFlat (env : evalEnvFlat) (c : fStates) :=
+    match c with
+    | (v, s) => do p <- nth_error (stateEnv env) v;
+                do s <- reifyStateSigmaFlat env s;
+                optReturn (flatPair flatstates flatStateSigma p s)
+    end. 
+
+  Definition reifyGammaFlat (env : evalEnvFlat) (c : fGamma) :=
+    match c with
+    | inl s => option_map (flatInl) (reifyStatesFlat env s)
+    | inr c => option_map (flatInr flatStates) (reifyTapeSigmaFlat env c)
+    end. 
+
+  Definition reifyPreludeSig'Flat (env : evalEnvFlat) (c : fpreludeSig') := 
+    match c with
+    | fnblank => optReturn flatNblank
+    | fnstar => optReturn flatNstar
+    | fninit => optReturn flatNinit
+    | fndelimC => optReturn flatNdelimC
+    | fnsigVar n => do s <- nth_error (sigmaEnv env) n;
+                    optReturn (flatNsig s)
+    end. 
+
+  Definition reifyAlphabetFlat (env : evalEnvFlat) (c : fAlphabet) := 
+    match c with 
+    | inl s => option_map (flatInl) (reifyGammaFlat env s)
+    | inr s => option_map (flatInr flatGamma) (reifyPreludeSig'Flat env s) 
+  end.  
+
+
